WIP

Phi_Logic_Programming_Reasoner/PLPR_error_msg.thy
@@ -20,43 +20,21 @@ consts literal_text :: \<open>(text \<Rightarrow> text) \<Rightarrow> text\<clos
 text \<open>We use the name of a lambda variable to encode an arbitrary string text.\<close>
 
 nonterminal "text_"
-syntax "_text_" :: \<open>text_ \<Rightarrow> text\<close> ("TEXT _" [1] 1000)
-syntax "_text_literal_" :: \<open>cartouche_position \<Rightarrow> text_\<close> ("_")
-syntax "_text_term_" :: \<open>logic \<Rightarrow> text_\<close> ("_" [1000] 2)
+syntax "_text_" :: \<open>text_ \<Rightarrow> text\<close> ("TEXT'(_')" [1] 1000)
+syntax "_text_literal_" :: \<open>cartouche \<Rightarrow> text_\<close> ("_")
+syntax "_text_term_" :: \<open>logic \<Rightarrow> text_\<close> ("_" [1000] 999)
 syntax "_text_cat_" :: \<open>text_ \<Rightarrow> text_ \<Rightarrow> text_\<close> ("_ _" [1,2] 1)
-
-declare [[ML_debugger]]
-
-parse_ast_translation \<open>
-let open Ast
-  fun dest_literal (Appl [Constant \<^syntax_const>\<open>_constrain\<close>, x, _]) = dest_literal x
-    | dest_literal (Appl [Constant \<^syntax_const>\<open>_text_literal_\<close>, x]) = dest_literal x
-    | dest_literal (Variable x) = String.substring (x, 7, size x - 15)
-        (*7 for size of \ <open> and 15 for size of \ <open> \ <close>*)
-  fun encode_literal str =
-    Appl [Constant \<^const_syntax>\<open>literal_text\<close>,
-    Appl [Constant \<^syntax_const>\<open>_abs\<close>,
-      Appl [Constant \<^syntax_const>\<open>_constrain\<close>, Variable str, Constant \<^type_syntax>\<open>text\<close>],
-      Appl [Constant \<^syntax_const>\<open>_constrain\<close>, Constant \<^const_syntax>\<open>undefined\<close>, Constant \<^type_syntax>\<open>text\<close>]]]
-  fun parse (Appl [Constant \<^syntax_const>\<open>_text_literal_\<close>, tm]) = encode_literal (dest_literal tm)
-    | parse (Appl [Constant \<^syntax_const>\<open>_text_term_\<close>, tm]) =
-        Appl [Constant \<^const_syntax>\<open>term_text\<close>, tm]
-    | parse (Appl [Constant \<^syntax_const>\<open>_text_cat_\<close>, tmA, tmB]) =
-        Appl [Constant \<^const_syntax>\<open>cat_text\<close>, parse tmA, parse tmB]
-in
-  [(\<^syntax_const>\<open>_text_\<close>, (fn ctxt => fn [ast] =>
-        Appl [Constant \<^const_syntax>\<open>text\<close>, parse ast]))]
-end\<close>
-
-term \<open>TEXT a b \<open>asd\<close> c \<open>asd\<close>\<close>
-
 
 ML \<open>
 structure Encode_Text = struct
+
+val escape_string   = String.translate (fn #"." => "\001" | x => str x)
+val recovery_string = String.translate (fn #"\001" => "." | x => str x)
+
 local open Ast
   fun dest_literal (Appl [Constant \<^syntax_const>\<open>_constrain\<close>, x, _]) = dest_literal x
     | dest_literal (Appl [Constant \<^syntax_const>\<open>_bound\<close>, x]) = dest_literal x
-    | dest_literal (Variable x) = x
+    | dest_literal (Variable x) = recovery_string x
 
 fun decode_text_ast' ret (Appl [Constant \<^const_syntax>\<open>literal_text\<close>,
       Appl [Constant \<^syntax_const>\<open>_abs\<close>, x, _]])
@@ -69,74 +47,103 @@ fun decode_text_ast' ret (Appl [Constant \<^const_syntax>\<open>literal_text\<cl
 
 in
 
-fun decode_text _ (\<^const>\<open>literal_text\<close> $ Abs (text, _, _)) = text
-  | decode_text ctxt (Const (\<^const_name>\<open>term_text\<close>, _) $ x) = Syntax.string_of_term ctxt x
+fun decode_text _ (\<^const>\<open>literal_text\<close> $ Abs (text, _, _)) = [Pretty.str (recovery_string text)]
+  | decode_text ctxt (Const (\<^const_name>\<open>term_text\<close>, _) $ x) = [Syntax.pretty_term ctxt x]
   | decode_text ctxt (\<^const>\<open>cat_text\<close> $ A $ B) =
-      decode_text ctxt A ^ " " ^ decode_text ctxt B
+      decode_text ctxt A @ decode_text ctxt B
   | decode_text ctxt (\<^const>\<open>text\<close> $ X) = decode_text ctxt X
   | decode_text _ tm = raise TERM ("decode_text", [tm])
+
+fun decode_text_str ctxt X =
+      Pretty.string_of (Pretty.block (Pretty.separate "" (decode_text ctxt X)))
 
 fun decode_text_ast ast =
   case decode_text_ast' [] ast
     of [] => Variable ""
      | [x] => x
      | l => Appl l
+
 end
 end
 \<close>
 
+parse_ast_translation \<open>
+let open Ast
+  fun dest_literal (Appl [Constant \<^syntax_const>\<open>_constrain\<close>, x, _]) = dest_literal x
+    | dest_literal (Appl [Constant \<^syntax_const>\<open>_text_literal_\<close>, x]) = dest_literal x
+    | dest_literal (Variable x) = String.substring (x, 7, size x - 15)
+        (*7 for size of \ <open> and 15 for size of \ <open> \ <close>*)
+  fun encode_literal str =
+    Appl [Constant \<^const_syntax>\<open>literal_text\<close>,
+    Appl [Constant \<^syntax_const>\<open>_abs\<close>,
+      Appl [Constant \<^syntax_const>\<open>_constrain\<close>,
+            Variable (Encode_Text.escape_string str),
+            Constant \<^type_syntax>\<open>text\<close>],
+      Appl [Constant \<^syntax_const>\<open>_constrain\<close>,
+            Constant \<^const_syntax>\<open>undefined\<close>,
+            Constant \<^type_syntax>\<open>text\<close>]]]
+  fun parse (Appl [Constant \<^syntax_const>\<open>_text_literal_\<close>, tm]) = encode_literal (dest_literal tm)
+    | parse (Appl [Constant \<^syntax_const>\<open>_text_term_\<close>, tm]) =
+        Appl [Constant \<^const_syntax>\<open>term_text\<close>, tm]
+    | parse (Appl [Constant \<^syntax_const>\<open>_text_cat_\<close>, tmA, tmB]) =
+        Appl [Constant \<^const_syntax>\<open>cat_text\<close>, parse tmA, parse tmB]
+in
+  [(\<^syntax_const>\<open>_text_\<close>, (fn ctxt => fn [ast] =>
+        Appl [Constant \<^const_syntax>\<open>text\<close>, parse ast]))]
+end\<close>
+
 print_ast_translation \<open>[(\<^const_syntax>\<open>text\<close>, (fn ctxt => fn [ast] =>
   Ast.Appl [Ast.Constant \<^syntax_const>\<open>_text_\<close>, Encode_Text.decode_text_ast ast]))]\<close>
+
 
 subsection \<open>Reasoners for Printing Message\<close>
 
 subsubsection \<open>Tracing\<close>
 
-definition TRACING :: \<open>text \<Rightarrow> prop\<close>
-  where \<open>TRACING x \<equiv> Trueprop True\<close>
+definition TRACING :: \<open>text \<Rightarrow> bool\<close>
+  where [iff]: \<open>TRACING x \<longleftrightarrow> True\<close>
 
-lemma TRACING_I: \<open>PROP TRACING x\<close>
+lemma TRACING_I: \<open>TRACING x\<close>
   unfolding TRACING_def ..
 
-\<phi>reasoner_ML TRACING 1200 (\<open>PROP TRACING ?x\<close>) = \<open>fn (ctxt,sequent) =>
+\<phi>reasoner_ML TRACING 1200 (\<open>TRACING ?x\<close>) = \<open>fn (ctxt,sequent) =>
   let
-    val \<^const>\<open>TRACING\<close> $ text = Thm.major_prem_of sequent
-    val str = Encode_Text.decode_text ctxt text
+    val \<^const>\<open>Trueprop\<close> $ (\<^const>\<open>TRACING\<close> $ text)
+          = Thm.major_prem_of sequent
+    val str = Encode_Text.decode_text_str ctxt text
     val _ = tracing str
   in Seq.single (ctxt, @{thm TRACING_I} RS sequent)
   end\<close>
 
 subsubsection \<open>Warning\<close>
 
-definition WARNING :: \<open>text \<Rightarrow> prop\<close>
-  where \<open>WARNING x \<equiv> Trueprop True\<close>
+definition WARNING :: \<open>text \<Rightarrow> bool\<close>
+  where [iff]: \<open>WARNING x \<longleftrightarrow> True\<close>
 
-lemma WARNING_I: \<open>PROP WARNING x\<close>
+lemma WARNING_I: \<open>WARNING x\<close>
   unfolding WARNING_def ..
 
-\<phi>reasoner_ML WARNING 1200 (\<open>PROP WARNING ?x\<close>) = \<open>fn (ctxt,sequent) =>
+\<phi>reasoner_ML WARNING 1200 (\<open>WARNING ?x\<close>) = \<open>fn (ctxt,sequent) =>
   let
-    val \<^const>\<open>WARNING\<close> $ text = Thm.major_prem_of sequent
-    val str = Encode_Text.decode_text ctxt text
+    val \<^const>\<open>Trueprop\<close> $ (\<^const>\<open>WARNING\<close> $ text)
+          = Thm.major_prem_of sequent
+    val str = Encode_Text.decode_text_str ctxt text
     val _ = warning str
   in Seq.single (ctxt, @{thm WARNING_I} RS sequent)
   end\<close>
 
 subsubsection \<open>Error\<close>
 
-definition ERROR :: \<open>text \<Rightarrow> prop\<close>
-  where \<open>ERROR x \<equiv> Trueprop True\<close>
+definition ERROR :: \<open>text \<Rightarrow> bool\<close>
+  where [iff]: \<open>ERROR x \<longleftrightarrow> False\<close>
 
-lemma ERROR_I: \<open>PROP ERROR x\<close>
-  unfolding ERROR_def ..
-
-\<phi>reasoner_ML ERROR 1200 (\<open>PROP ERROR ?x\<close>) = \<open>fn (ctxt,sequent) =>
+\<phi>reasoner_ML ERROR 1200 (\<open>ERROR ?x\<close>) = \<open>fn (ctxt,sequent) =>
   let
-    val \<^const>\<open>ERROR\<close> $ text = Thm.major_prem_of sequent
-    val str = Encode_Text.decode_text ctxt text
+    val \<^const>\<open>Trueprop\<close> $ (\<^const>\<open>ERROR\<close> $ text)
+          = Thm.major_prem_of sequent
+    val str = Encode_Text.decode_text_str ctxt text
     val _ = error str
-  in Seq.single (ctxt, @{thm ERROR_I} RS sequent)
+  in Seq.empty
   end\<close>
-
 
 end
