Phi_Semantics/PhiSem_Variable_Lib.thy
@@ -1,44 +1,23 @@
 theory PhiSem_Variable_Lib
-  imports PhiSem_Variable
+  imports PhiSem_Typed_Variable
 begin
 
 section \<open>Basic Operations\<close>
 
 subsection \<open>Variable\<close>
 
+
+proc
+  argument \<open>x \<Ztypecolon> \<^bold>v\<^bold>a\<^bold>l T\<heavy_comma> y \<Ztypecolon> \<^bold>v\<^bold>a\<^bold>l U\<close>
+  return \<open>xxxx\<close>
+  \<medium_left_bracket>
+  ;; \<open>$1\<close> \<open>$1\<close>
+  ;; \<open>$2 := xx\<close>
+
 subsubsection \<open>Syntax\<close>
 
-syntax "__var__" :: "idt \<Rightarrow> logic" ("\<^bold>v\<^bold>a\<^bold>r _" [1000] 999)
-
-parse_ast_translation \<open>
-  let open Ast
-    fun mk_Var name =
-      Appl [Constant \<^const_syntax>\<open>\<phi>Type\<close>, Constant \<^const_syntax>\<open>Pure.dummy_pattern\<close>,
-        Appl [Variable "Var", name, Constant \<^const_syntax>\<open>Pure.dummy_pattern\<close>]]
-   in [(\<^syntax_const>\<open>__var__\<close>, fn ctxt => fn [name] => mk_Var name)]
-  end
-\<close>
-
-syntax "__get_var__" :: "idt \<Rightarrow> logic" ("$_" [1000] 999)
-consts "get_var____\<phi>" :: "varname \<Rightarrow> 'b"
-
-translations "$x" => "CONST get_var____\<phi> x"
-
-definition Variable_of :: \<open>'a \<Rightarrow> varname \<Rightarrow> 'a\<close> (infix "<val-of-var>" 22)
-  where [iff]: \<open>(S <val-of-var> V) = S\<close>
-
-definition Set_Variable :: \<open>varname \<Rightarrow> 'a \<Rightarrow> 'a\<close> ("$_ := _" [1000, 51] 50)
-  where [iff]: \<open>($x := y) = y\<close>
-
-lemma [\<phi>reason 2000 for
-  \<open>Synthesis_Parse (?var::varname) (?Y::?'ret \<Rightarrow> assn)\<close>
-]:
-  \<open>Synthesis_Parse var (\<lambda>_. x \<Ztypecolon> Var var T :: assn)\<close>
-  unfolding Synthesis_Parse_def ..
-
-
-\<phi>processor get_variable 5000 (\<open>\<^bold>c\<^bold>u\<^bold>r\<^bold>r\<^bold>e\<^bold>n\<^bold>t ?blk [?H] \<^bold>r\<^bold>e\<^bold>s\<^bold>u\<^bold>l\<^bold>t\<^bold>s \<^bold>i\<^bold>n ?T\<close>)  \<open>
-  fn (ctxt,sequent) => \<^keyword>\<open>$\<close> |-- Parse.term >> (fn var => fn () =>
+\<phi>processor decl_variable 5000 (\<open>\<^bold>c\<^bold>u\<^bold>r\<^bold>r\<^bold>e\<^bold>n\<^bold>t ?blk [?H] \<^bold>r\<^bold>e\<^bold>s\<^bold>u\<^bold>l\<^bold>t\<^bold>s \<^bold>i\<^bold>n ?T\<close>)  \<open>
+  fn (ctxt,sequent) => \<^keyword>\<open>var\<close> |-- Parse.term >> (fn var => fn () =>
     let
       val ctxt_parse = Config.put phi_synthesis_parsing true ctxt
       val term = Const(\<^const_name>\<open>get_var____\<phi>\<close>, dummyT) $ Syntax.parse_term ctxt_parse var
@@ -50,22 +29,48 @@ lemma [\<phi>reason 2000 for
 \<close>
 
 
+(*
+syntax "__var__" :: "idt \<Rightarrow> logic" ("\<^bold>v\<^bold>a\<^bold>r _" [1000] 999)
+
+parse_ast_translation \<open>
+  let open Ast
+    fun mk_Var name =
+      Appl [Constant \<^const_syntax>\<open>\<phi>Type\<close>, Constant \<^const_syntax>\<open>Pure.dummy_pattern\<close>,
+        Appl [Variable "Var", name, Constant \<^const_syntax>\<open>Pure.dummy_pattern\<close>]]
+   in [(\<^syntax_const>\<open>__var__\<close>, fn ctxt => fn [name] => mk_Var name)]
+  end
+\<close> *)
+
+syntax "__get_var__" :: "idt \<Rightarrow> logic" ("$_" [1000] 999)
+consts "get_var____\<phi>" :: "varname \<Rightarrow> 'b"
+
+translations "$x" => "CONST get_var____\<phi> x"
+
+
+lemma [\<phi>reason 2000 for
+  \<open>Synthesis_Parse (?var::varname) (?Y::?'ret \<Rightarrow> assn)\<close>
+]:
+  \<open>Synthesis_Parse var (\<lambda>_. x \<Ztypecolon> Var var T :: assn)\<close>
+  unfolding Synthesis_Parse_def ..
+
+
+
 subsubsection \<open>Operations\<close>
 
 paragraph \<open>Get Variable\<close>
 
 proc (nodef) op_get_var:
   assumes [unfolded \<phi>SemType_def subset_iff, useful]: \<open>\<phi>SemType (x \<Ztypecolon> T) TY\<close>
-  argument \<open>x \<Ztypecolon> Var vname T\<close>
-  return   \<open>x \<Ztypecolon> Var vname T\<heavy_comma> \<^bold>v\<^bold>a\<^bold>l x \<Ztypecolon> T\<close>
+  argument \<open>x \<Ztypecolon> \<^bold>v\<^bold>a\<^bold>r[var] T\<close>
+  return   \<open>x \<Ztypecolon> \<^bold>v\<^bold>a\<^bold>r[var] T\<heavy_comma> x \<Ztypecolon> \<^bold>v\<^bold>a\<^bold>l T\<close>
   \<medium_left_bracket> to_Identity op_get_var'' \<medium_right_bracket> using \<phi> by simp .
 
-lemma [\<phi>reason for \<open>\<^bold>p\<^bold>r\<^bold>o\<^bold>c ?f \<lbrace> ?R \<longmapsto> \<lambda>ret. ?R'\<heavy_comma> SYNTHESIS ?x <val-of-var> ?var \<Ztypecolon> ?T ret \<^bold>t\<^bold>h\<^bold>r\<^bold>o\<^bold>w\<^bold>s ?E \<rbrace> \<^bold>@\<^bold>G\<^bold>O\<^bold>A\<^bold>L ?G\<close>]:
+lemma [\<phi>reason for \<open>\<^bold>p\<^bold>r\<^bold>o\<^bold>c ?f \<lbrace> ?R \<longmapsto> \<lambda>ret. ?R'\<heavy_comma> SYNTHESIS ?x <val-of> ?var \<Ztypecolon> ?T ret \<^bold>t\<^bold>h\<^bold>r\<^bold>o\<^bold>w\<^bold>s ?E \<rbrace> \<^bold>@\<^bold>G\<^bold>O\<^bold>A\<^bold>L ?G\<close>]:
   \<open> SUBGOAL G G2
-\<Longrightarrow> \<^bold>v\<^bold>i\<^bold>e\<^bold>w X \<longmapsto> Y\<heavy_comma> \<blangle> x \<Ztypecolon> Var var T \<brangle> \<^bold><\<^bold>a\<^bold>c\<^bold>t\<^bold>i\<^bold>o\<^bold>n\<^bold>> ToSA \<^bold>@\<^bold>G\<^bold>O\<^bold>A\<^bold>L G2
+\<Longrightarrow> \<^bold>v\<^bold>i\<^bold>e\<^bold>w X \<longmapsto> Y\<heavy_comma> \<blangle> x \<Ztypecolon> \<^bold>v\<^bold>a\<^bold>r[var] T \<brangle> \<^bold><\<^bold>a\<^bold>c\<^bold>t\<^bold>i\<^bold>o\<^bold>n\<^bold>> ToSA \<^bold>@\<^bold>G\<^bold>O\<^bold>A\<^bold>L G2
 \<Longrightarrow> SOLVE_SUBGOAL G2
 \<Longrightarrow> \<phi>SemType (x \<Ztypecolon> T) TY
-\<Longrightarrow> \<^bold>p\<^bold>r\<^bold>o\<^bold>c op_get_var var TY \<lbrace> X \<longmapsto> Y\<heavy_comma> x \<Ztypecolon> Var var T \<heavy_comma> SYNTHESIS \<^bold>v\<^bold>a\<^bold>l x <val-of-var> var \<Ztypecolon> T \<rbrace> \<^bold>@\<^bold>G\<^bold>O\<^bold>A\<^bold>L G\<close>
+\<Longrightarrow> \<^bold>p\<^bold>r\<^bold>o\<^bold>c op_get_var var TY \<lbrace> X \<longmapsto> Y\<heavy_comma> x \<Ztypecolon> \<^bold>v\<^bold>a\<^bold>r[var] T \<heavy_comma> SYNTHESIS \<^bold>v\<^bold>a\<^bold>l x <val-of> var \<Ztypecolon> T \<rbrace> \<^bold>@\<^bold>G\<^bold>O\<^bold>A\<^bold>L G\<close>
   unfolding Action_Tag_def
   \<medium_left_bracket> premises _ and GetVar and _ and [\<phi>reason for \<open>\<phi>SemType (x \<Ztypecolon> T) ?TY\<close>]
     GetVar op_get_var \<medium_right_bracket>. .
@@ -74,26 +79,51 @@ lemma [\<phi>reason for \<open>\<^bold>p\<^bold>r\<^bold>o\<^bold>c ?f \<lbrace>
 
 paragraph \<open>Set Variable\<close>
 
+consts infer_var_type :: \<open>unit action\<close>
+
+lemma [\<phi>reason 1000]:
+  \<open> varname.type var \<equiv> TY'
+\<Longrightarrow> pred_option (\<lambda>TY'. TY = TY') TY' \<^bold><\<^bold>a\<^bold>c\<^bold>t\<^bold>i\<^bold>o\<^bold>n\<^bold>> infer_var_type
+\<Longrightarrow> pred_option (\<lambda>TY'. TY = TY') (varname.type var) \<^bold><\<^bold>a\<^bold>c\<^bold>t\<^bold>i\<^bold>o\<^bold>n\<^bold>> infer_var_type\<close>
+  \<comment> \<open>TY is the output. The rule invokes evaluation of the \<open>varname.type var\<close>.\<close>
+  by simp
+
+lemma [\<phi>reason 1000]:
+  \<open>pred_option (\<lambda>TY'. TY = TY') None \<^bold><\<^bold>a\<^bold>c\<^bold>t\<^bold>i\<^bold>o\<^bold>n\<^bold>> infer_var_type\<close>
+  \<comment> \<open>the output TY can be anything freely\<close>
+  by simp
+
+lemma [\<phi>reason 1000]:
+  \<open>pred_option (\<lambda>TY'. TY = TY') (Some TY) \<^bold><\<^bold>a\<^bold>c\<^bold>t\<^bold>i\<^bold>o\<^bold>n\<^bold>> infer_var_type\<close>
+  \<comment> \<open>the output TY equals to that TY in \<open>Some TY\<close> exactly.\<close>
+  by simp
+
+lemma
+  \<open>pred_option (\<lambda>TY'. TY = TY') None\<close>
+  \<open>pred_option (\<lambda>TY'. TY = TY') (Some TY)\<close>
+  by simp+
+
 proc (nodef) op_set_var:
-  assumes [unfolded \<phi>SemType_def subset_iff, useful]: \<open>\<phi>SemType (x \<Ztypecolon> T) TY\<close>
-  assumes [unfolded \<phi>SemType_def subset_iff, useful]: \<open>\<phi>SemType (y \<Ztypecolon> U) TY\<close>
+  assumes [unfolded Action_Tag_def, useful]:
+      \<open>pred_option (\<lambda>TY'. TY = TY') (varname.type var) \<^bold><\<^bold>a\<^bold>c\<^bold>t\<^bold>i\<^bold>o\<^bold>n\<^bold>> infer_var_type\<close>
+  assumes [unfolded \<phi>SemType_def subset_iff, useful]:
+      \<open>\<phi>SemType (y \<Ztypecolon> U) TY\<close>
   argument \<open>x \<Ztypecolon> Var var T\<heavy_comma> \<^bold>v\<^bold>a\<^bold>l y \<Ztypecolon> U\<close>
-  return   \<open>y \<Ztypecolon> Var var U\<close>
+  return   \<open>y \<Ztypecolon> \<^bold>v\<^bold>a\<^bold>r[var] U\<close>
   \<medium_left_bracket> to_Identity \<open>var\<close> to_Identity op_set_var'' \<medium_right_bracket>. .
 
-proc (nodef) op_set_var__synthesis[
+schematic_goal op_set_var__synthesis[
   \<phi>reason for \<open>\<^bold>p\<^bold>r\<^bold>o\<^bold>c ?f \<lbrace> ?R \<longmapsto> \<lambda>ret. ?R'\<heavy_comma> SYNTHESIS ($?var := ?y) \<Ztypecolon> ?U ret \<^bold>t\<^bold>h\<^bold>r\<^bold>o\<^bold>w\<^bold>s ?E \<rbrace> \<^bold>@\<^bold>G\<^bold>O\<^bold>A\<^bold>L ?G\<close>
 ]:
 assumes G: \<open>\<^bold>p\<^bold>r\<^bold>o\<^bold>c g \<lbrace> X \<longmapsto> X1\<heavy_comma> SYNTHESIS \<^bold>v\<^bold>a\<^bold>l y \<Ztypecolon> U \<^bold>t\<^bold>h\<^bold>r\<^bold>o\<^bold>w\<^bold>s E\<rbrace> \<^bold>@\<^bold>G\<^bold>O\<^bold>A\<^bold>L G \<close>
   and S[unfolded Action_Tag_def]:
-        \<open>\<And>vy. \<^bold>v\<^bold>i\<^bold>e\<^bold>w X1\<heavy_comma> y \<Ztypecolon> Val vy U \<longmapsto> Y\<heavy_comma> x \<Ztypecolon> Var var T\<heavy_comma> y \<Ztypecolon> Val vy U \<^bold>w\<^bold>i\<^bold>t\<^bold>h Any \<^bold><\<^bold>a\<^bold>c\<^bold>t\<^bold>i\<^bold>o\<^bold>n\<^bold>> ToSA\<close>
-  and [\<phi>reason for \<open>\<phi>SemType (x \<Ztypecolon> T) ?TY\<close>]: \<open>\<phi>SemType (x \<Ztypecolon> T) TY\<close>
-  and [\<phi>reason for \<open>\<phi>SemType (y \<Ztypecolon> U) ?TY\<close>]: \<open>\<phi>SemType (y \<Ztypecolon> U) TY\<close>
- goal G
-argument \<open>X\<close>
-return   \<open>Y\<heavy_comma> y \<Ztypecolon> Var var U \<heavy_comma> SYNTHESIS \<^bold>v\<^bold>a\<^bold>l ($var := y) \<Ztypecolon> U\<close>
-throws   E
-  \<medium_left_bracket> G S op_set_var op_get_var \<medium_right_bracket>. .
+         \<open>\<And>vy. \<^bold>v\<^bold>i\<^bold>e\<^bold>w X1\<heavy_comma> y \<Ztypecolon> Val vy U \<longmapsto> Y\<heavy_comma> x \<Ztypecolon> Var var T\<heavy_comma> y \<Ztypecolon> Val vy U \<^bold>w\<^bold>i\<^bold>t\<^bold>h Any \<^bold><\<^bold>a\<^bold>c\<^bold>t\<^bold>i\<^bold>o\<^bold>n\<^bold>> ToSA\<close>
+  and P: \<open>pred_option (\<lambda>TY'. TY = TY') (varname.type var) \<^bold><\<^bold>a\<^bold>c\<^bold>t\<^bold>i\<^bold>o\<^bold>n\<^bold>> infer_var_type\<close>
+  and [\<phi>reason for \<open>\<phi>SemType (y \<Ztypecolon> U) ?TY\<close>]:
+         \<open>\<phi>SemType (y \<Ztypecolon> U) TY\<close>
+shows \<open>\<^bold>p\<^bold>r\<^bold>o\<^bold>c ?FF \<lbrace> X \<longmapsto> Y\<heavy_comma> y \<Ztypecolon> \<^bold>v\<^bold>a\<^bold>r[var] U \<heavy_comma> SYNTHESIS \<^bold>v\<^bold>a\<^bold>l ($var := y) \<Ztypecolon> U \<^bold>t\<^bold>h\<^bold>r\<^bold>o\<^bold>w\<^bold>s E \<rbrace> \<^bold>@\<^bold>G\<^bold>O\<^bold>A\<^bold>L G\<close>
+  \<medium_left_bracket> G S op_set_var P op_get_var \<medium_right_bracket>. .
+
 
 
 paragraph \<open>Declare New Variables\<close>
@@ -102,38 +132,38 @@ paragraph \<open>Declare New Variables\<close>
 declare [[ML_print_depth=1000, eta_contract=false]]
 
 proc op_var_scope:
-  assumes [unfolded \<phi>SemType_def subset_iff, useful]: \<open>\<phi>SemType (x \<Ztypecolon> T) TY\<close>
-    and BLK: \<open>\<forall>var. \<^bold>p\<^bold>r\<^bold>o\<^bold>c F var \<lbrace> X\<heavy_comma> x \<Ztypecolon> Var var T \<longmapsto> \<lambda>ret. Y ret\<heavy_comma> () \<Ztypecolon> Var var (\<phi>Any <of-type> TY)
-                    \<^bold>t\<^bold>h\<^bold>r\<^bold>o\<^bold>w\<^bold>s \<lambda>v. E v \<heavy_comma> () \<Ztypecolon> Var var (\<phi>Any <of-type> TY) \<rbrace>\<close>
-  argument \<open>X\<heavy_comma> \<^bold>v\<^bold>a\<^bold>l x \<Ztypecolon> T\<close>
+  assumes BLK: \<open>\<And>var. varname.type var \<equiv> TY
+                  \<Longrightarrow> \<^bold>p\<^bold>r\<^bold>o\<^bold>c F var \<lbrace> X\<heavy_comma> \<^bold>u\<^bold>n\<^bold>i\<^bold>n\<^bold>i\<^bold>t\<^bold>e\<^bold>d \<^bold>v\<^bold>a\<^bold>r[var] \<longmapsto> \<lambda>ret. Y ret\<heavy_comma> () \<Ztypecolon> Var var \<phi>Any
+                      \<^bold>t\<^bold>h\<^bold>r\<^bold>o\<^bold>w\<^bold>s \<lambda>v. E v \<heavy_comma> () \<Ztypecolon> Var var \<phi>Any \<rbrace>\<close>
+  argument \<open>X\<close>
   return   \<open>Y\<close>
   throws   E
-  \<medium_left_bracket> to_Identity op_var_scope'
-    try'' \<medium_left_bracket> BLK to_Identity op_free_var \<medium_right_bracket>. \<medium_left_bracket> to_Identity op_free_var throw \<medium_right_bracket>. \<medium_right_bracket>. .
-
-lemma "__\<phi>op_var_scope__":
-  \<open> (\<And>var. \<^bold>p\<^bold>r\<^bold>o\<^bold>c F var \<lbrace> R\<heavy_comma> x \<Ztypecolon> Var var T\<heavy_comma>  X \<longmapsto> \<lambda>ret. Y ret \<heavy_comma> () \<Ztypecolon> Var var (\<phi>Any <of-type> TY)
-                \<^bold>t\<^bold>h\<^bold>r\<^bold>o\<^bold>w\<^bold>s \<lambda>v. E v \<heavy_comma> () \<Ztypecolon> Var var (\<phi>Any <of-type> TY) \<rbrace>)
-\<Longrightarrow> \<phi>SemType (x \<Ztypecolon> T) TY
-\<Longrightarrow> \<^bold>p\<^bold>r\<^bold>o\<^bold>c op_var_scope TYPE('a) TY F raw \<lbrace> R\<heavy_comma> (X\<heavy_comma> x \<Ztypecolon> Val raw T) \<longmapsto> \<lambda>ret. Y ret \<^bold>t\<^bold>h\<^bold>r\<^bold>o\<^bold>w\<^bold>s E \<rbrace>\<close>
-  unfolding mult.assoc[symmetric]
-  using op_var_scope_\<phi>app[where X=\<open>R\<heavy_comma> X\<close> and x = x and T = T and TY = TY and F=F,
-            of Y E \<open>raw\<close>, simplified]
-  by (smt (verit, best) ab_semigroup_mult_class.mult_ac(1) mult.commute)
+  \<medium_left_bracket> op_var_scope'[where TY=TY]
+    try''
+    \<medium_left_bracket> premises [\<phi>reason]
+      BLK to_Identity op_free_var
+    \<medium_right_bracket>.
+    \<medium_left_bracket> to_Identity op_free_var throw \<medium_right_bracket>.
+  \<medium_right_bracket>. .
 
 lemma "__\<phi>op_set_var__":
-  \<open> \<^bold>p\<^bold>r\<^bold>o\<^bold>c g \<lbrace> R\<heavy_comma> y \<Ztypecolon> Var var U\<heavy_comma> X \<longmapsto> Z \<^bold>t\<^bold>h\<^bold>r\<^bold>o\<^bold>w\<^bold>s E \<rbrace>
-\<Longrightarrow> \<phi>SemType (x \<Ztypecolon> T) TY
+  \<open> \<^bold>p\<^bold>r\<^bold>o\<^bold>c g \<lbrace> R\<heavy_comma> y \<Ztypecolon> \<^bold>v\<^bold>a\<^bold>r[var] U\<heavy_comma> X \<longmapsto> Z \<^bold>t\<^bold>h\<^bold>r\<^bold>o\<^bold>w\<^bold>s E \<rbrace>
+\<Longrightarrow> pred_option (\<lambda>TY'. TY = TY') (varname.type var) \<^bold><\<^bold>a\<^bold>c\<^bold>t\<^bold>i\<^bold>o\<^bold>n\<^bold>> infer_var_type
 \<Longrightarrow> \<phi>SemType (y \<Ztypecolon> U) TY
 \<Longrightarrow> \<^bold>p\<^bold>r\<^bold>o\<^bold>c (op_set_var var TY raw \<ggreater> g) \<lbrace> R\<heavy_comma> (X\<heavy_comma> x \<Ztypecolon> Var var T \<heavy_comma> y \<Ztypecolon> Val raw U) \<longmapsto> Z \<^bold>t\<^bold>h\<^bold>r\<^bold>o\<^bold>w\<^bold>s E \<rbrace>\<close>
-  \<medium_left_bracket> premises G and [\<phi>reason for \<open>\<phi>SemType (x \<Ztypecolon> T) ?TY\<close>] and [\<phi>reason for \<open>\<phi>SemType (y \<Ztypecolon> U) ?TY\<close>]
-    op_set_var G \<medium_right_bracket>. .
-
+  \<medium_left_bracket> premises G and P and [\<phi>reason for \<open>\<phi>SemType (y \<Ztypecolon> U) ?TY\<close>]
+    op_set_var P G \<medium_right_bracket>. .
 
 lemma "__\<phi>op_var_scope__0":
   \<open> \<^bold>p\<^bold>r\<^bold>o\<^bold>c F \<lbrace> R \<longmapsto> Y \<^bold>t\<^bold>h\<^bold>r\<^bold>o\<^bold>w\<^bold>s E \<rbrace>
 \<Longrightarrow> \<^bold>p\<^bold>r\<^bold>o\<^bold>c F \<lbrace> R\<heavy_comma> Void \<longmapsto> Y \<^bold>t\<^bold>h\<^bold>r\<^bold>o\<^bold>w\<^bold>s E \<rbrace>\<close>
   by fastforce
+
+
+thm "__\<phi>op_set_var__"[OF "__\<phi>op_set_var__" [OF "__\<phi>op_var_scope__0"]]
+
+term \<open>x.x.x.x := xx\<close>
+
 
 ML_file_debug "library/local_value.ML"
 
