Phi_Semantics/PhiSem_Play_Ground.thy
@@ -41,5 +41,5 @@ proc
     $v
   \<medium_right_bracket>. .
 
-
+  
 end
