Phi_System/IDE_CP_Applications.thy
@@ -1,9 +1,0 @@
-chapter \<open>More Pre-built Applications\<close>
-
-theory IDE_CP_Applications
-  imports IDE_CP_Reasoning
-begin
-
-
-
-end
