Phi_System/IDE_CP_Applications1.thy
@@ -1,0 +1,166 @@
+chapter \<open>IDE-CP Functions \& Applications - Part I\<close>
+
+text \<open>In this part, we build simple applications based on IDE-CP directly, without too much
+  advanced reasoning processes.\<close>
+
+theory IDE_CP_Applications1
+  imports Phi_Types
+begin
+
+section \<open>Value \& Its Settings\<close>
+
+subsection \<open>Reasoning Rules\<close>
+
+paragraph \<open>Implication\<close>
+
+lemma Val_cast [\<phi>reason]:
+  \<open> y \<Ztypecolon> U \<^bold>i\<^bold>m\<^bold>p\<^bold>l\<^bold>i\<^bold>e\<^bold>s x \<Ztypecolon> T \<^bold>a\<^bold>n\<^bold>d P
+\<Longrightarrow> y \<Ztypecolon> Val v U \<^bold>i\<^bold>m\<^bold>p\<^bold>l\<^bold>i\<^bold>e\<^bold>s x \<Ztypecolon> Val v T \<^bold>a\<^bold>n\<^bold>d P\<close>
+  unfolding Imply_def by (simp add: \<phi>expns)
+
+paragraph \<open>Action\<close>
+
+lemma [\<phi>reason 1200 for \<open>?y \<Ztypecolon> Val ?v ?U \<^bold>i\<^bold>m\<^bold>p\<^bold>l\<^bold>i\<^bold>e\<^bold>s ?T \<^bold>a\<^bold>n\<^bold>d ?P \<^bold><\<^bold>a\<^bold>c\<^bold>t\<^bold>i\<^bold>o\<^bold>n\<^bold>> (?Act::?'a::structural action)\<close>]:
+  \<open> y \<Ztypecolon> U \<^bold>i\<^bold>m\<^bold>p\<^bold>l\<^bold>i\<^bold>e\<^bold>s x \<Ztypecolon> T \<^bold>a\<^bold>n\<^bold>d P \<^bold><\<^bold>a\<^bold>c\<^bold>t\<^bold>i\<^bold>o\<^bold>n\<^bold>> Act
+\<Longrightarrow> y \<Ztypecolon> Val v U \<^bold>i\<^bold>m\<^bold>p\<^bold>l\<^bold>i\<^bold>e\<^bold>s x \<Ztypecolon> Val v T \<^bold>a\<^bold>n\<^bold>d P \<^bold><\<^bold>a\<^bold>c\<^bold>t\<^bold>i\<^bold>o\<^bold>n\<^bold>> Act\<close>
+  for Act :: \<open>'a::structural action\<close>
+  unfolding Action_Tag_def
+  using Val_cast .
+
+paragraph \<open>Simplification\<close>
+
+lemma [\<phi>programming_simps]:
+    \<open>Val raw (ExTyp T) = (\<exists>\<phi> c. Val raw (T c))\<close>
+  by (rule \<phi>Type_eqI) (simp add: \<phi>expns)
+
+lemma [\<phi>programming_simps]:
+    \<open>Val raw (T \<phi>\<^bold>s\<^bold>u\<^bold>b\<^bold>j P) = (Val raw T \<phi>\<^bold>s\<^bold>u\<^bold>b\<^bold>j P)\<close>
+  by (rule \<phi>Type_eqI) (simp add: \<phi>expns)
+
+lemma \<phi>Val_simp_cong[folded atomize_eq]:
+  \<open> (x \<Ztypecolon> T) = (x' \<Ztypecolon> T')
+\<Longrightarrow> (x \<Ztypecolon> Val v T) = (x' \<Ztypecolon> Val v T')\<close>
+  unfolding set_eq_iff by (simp add: \<phi>expns)
+
+simproc_setup Val_simp_cong ("x \<Ztypecolon> Val v T") = \<open>
+  K (fn ctxt => Phi_SimpCong.simproc @{thm \<phi>Val_simp_cong} ctxt)
+\<close>
+
+subsection \<open>Application Methods for Transformations\<close>
+
+(*TODO: I really don't like this. It is not generic.
+It should be some generic structural morphism.*)
+
+lemma [\<phi>reason 2100 for \<open>
+  PROP \<phi>Application_Method (Trueprop (?x \<Ztypecolon> ?T \<^bold>i\<^bold>m\<^bold>p\<^bold>l\<^bold>i\<^bold>e\<^bold>s ?y \<Ztypecolon> ?U \<^bold>a\<^bold>n\<^bold>d ?P))
+          (Trueprop (\<^bold>c\<^bold>u\<^bold>r\<^bold>r\<^bold>e\<^bold>n\<^bold>t ?blk [?RR] \<^bold>r\<^bold>e\<^bold>s\<^bold>u\<^bold>l\<^bold>t\<^bold>s \<^bold>i\<^bold>n ?R\<heavy_comma> ?x \<Ztypecolon> Val ?raw ?T)) ?Result
+\<close> except \<open>
+  PROP \<phi>Application_Method (Trueprop (?x \<Ztypecolon> Val ?raw ?T \<^bold>i\<^bold>m\<^bold>p\<^bold>l\<^bold>i\<^bold>e\<^bold>s ?y \<Ztypecolon> ?U \<^bold>a\<^bold>n\<^bold>d ?P))
+          (Trueprop (\<^bold>c\<^bold>u\<^bold>r\<^bold>r\<^bold>e\<^bold>n\<^bold>t ?blk [?RR] \<^bold>r\<^bold>e\<^bold>s\<^bold>u\<^bold>l\<^bold>t\<^bold>s \<^bold>i\<^bold>n ?R)) ?Result
+\<close>]:
+  \<open> PROP \<phi>Application_Success
+\<Longrightarrow> PROP \<phi>Application_Method (Trueprop (x \<Ztypecolon> T \<^bold>i\<^bold>m\<^bold>p\<^bold>l\<^bold>i\<^bold>e\<^bold>s y \<Ztypecolon> U \<^bold>a\<^bold>n\<^bold>d P))
+      (Trueprop (\<^bold>c\<^bold>u\<^bold>r\<^bold>r\<^bold>e\<^bold>n\<^bold>t blk [RR] \<^bold>r\<^bold>e\<^bold>s\<^bold>u\<^bold>l\<^bold>t\<^bold>s \<^bold>i\<^bold>n R\<heavy_comma> x \<Ztypecolon> Val raw T))
+      (Trueprop ((\<^bold>c\<^bold>u\<^bold>r\<^bold>r\<^bold>e\<^bold>n\<^bold>t blk [RR] \<^bold>r\<^bold>e\<^bold>s\<^bold>u\<^bold>l\<^bold>t\<^bold>s \<^bold>i\<^bold>n R\<heavy_comma> y \<Ztypecolon> Val raw U) \<and> P))\<close>
+  unfolding \<phi>Application_Method_def \<phi>Application_def
+  using "\<phi>cast_P" Val_cast implies_left_prod by metis
+
+
+lemma [\<phi>reason 2000 for \<open>
+  PROP \<phi>Application_Method (Trueprop (?x' \<Ztypecolon> ?T' \<^bold>i\<^bold>m\<^bold>p\<^bold>l\<^bold>i\<^bold>e\<^bold>s ?y \<Ztypecolon> ?U \<^bold>a\<^bold>n\<^bold>d ?P))
+      (Trueprop (\<^bold>c\<^bold>u\<^bold>r\<^bold>r\<^bold>e\<^bold>n\<^bold>t ?blk [?RR] \<^bold>r\<^bold>e\<^bold>s\<^bold>u\<^bold>l\<^bold>t\<^bold>s \<^bold>i\<^bold>n ?R\<heavy_comma> ?x \<Ztypecolon> Val ?raw ?T)) ?Result
+\<close> except \<open>
+  PROP \<phi>Application_Method (Trueprop (?x \<Ztypecolon> Val ?raw ?T \<^bold>i\<^bold>m\<^bold>p\<^bold>l\<^bold>i\<^bold>e\<^bold>s ?y \<Ztypecolon> ?U \<^bold>a\<^bold>n\<^bold>d ?P))
+          (Trueprop (\<^bold>c\<^bold>u\<^bold>r\<^bold>r\<^bold>e\<^bold>n\<^bold>t ?blk [?RR] \<^bold>r\<^bold>e\<^bold>s\<^bold>u\<^bold>l\<^bold>t\<^bold>s \<^bold>i\<^bold>n ?R)) ?Result
+\<close>]:
+  \<open> SUBGOAL TOP_GOAL G
+\<Longrightarrow> x \<Ztypecolon> T \<^bold>i\<^bold>m\<^bold>p\<^bold>l\<^bold>i\<^bold>e\<^bold>s x' \<Ztypecolon> T' \<^bold>a\<^bold>n\<^bold>d Any
+\<Longrightarrow> SOLVE_SUBGOAL G
+\<Longrightarrow> PROP \<phi>Application_Success
+\<Longrightarrow> \<^bold>o\<^bold>b\<^bold>l\<^bold>i\<^bold>g\<^bold>a\<^bold>t\<^bold>i\<^bold>o\<^bold>n True
+\<Longrightarrow> PROP \<phi>Application_Method (Trueprop (x' \<Ztypecolon> T' \<^bold>i\<^bold>m\<^bold>p\<^bold>l\<^bold>i\<^bold>e\<^bold>s y \<Ztypecolon> U \<^bold>a\<^bold>n\<^bold>d P))
+      (Trueprop (\<^bold>c\<^bold>u\<^bold>r\<^bold>r\<^bold>e\<^bold>n\<^bold>t blk [RR] \<^bold>r\<^bold>e\<^bold>s\<^bold>u\<^bold>l\<^bold>t\<^bold>s \<^bold>i\<^bold>n R\<heavy_comma> x \<Ztypecolon> Val raw T))
+      (Trueprop ((\<^bold>c\<^bold>u\<^bold>r\<^bold>r\<^bold>e\<^bold>n\<^bold>t blk [RR] \<^bold>r\<^bold>e\<^bold>s\<^bold>u\<^bold>l\<^bold>t\<^bold>s \<^bold>i\<^bold>n R\<heavy_comma> y \<Ztypecolon> Val raw U) \<and> P))\<close>
+  unfolding \<phi>Application_Method_def \<phi>Application_def
+  using "\<phi>cast_P" Val_cast implies_left_prod by metis
+
+
+subsection \<open>Synthesis\<close>
+
+lemma [\<phi>reason 1200 for
+  \<open>Synthesis_Parse (?x \<Ztypecolon> (?T::?'a \<Rightarrow> VAL set)) (?X::?'ret \<Rightarrow> assn)\<close>
+]:
+  \<open>Synthesis_Parse (x \<Ztypecolon> T) (\<lambda>v. x \<Ztypecolon> Val v T)\<close>
+  unfolding Synthesis_Parse_def ..
+
+lemma [\<phi>reason 1200 for
+  \<open>Synthesis_Parse (?raw::?'a sem_value) (?X::?'ret \<Rightarrow> assn)\<close>
+]:
+  \<open>Synthesis_Parse raw (\<lambda>_. x \<Ztypecolon> Val raw T)\<close>
+  unfolding Synthesis_Parse_def ..
+
+lemma [\<phi>reason 1200 for \<open>\<^bold>v\<^bold>i\<^bold>e\<^bold>w ?S1 \<longmapsto> ?S2\<heavy_comma> SYNTHESIS ?x \<Ztypecolon> Val ?raw ?T  \<^bold>@\<^bold>G\<^bold>O\<^bold>A\<^bold>L ?G\<close>]:
+  \<open> sem_value.dest raw \<in> (x \<Ztypecolon> T)
+\<Longrightarrow> \<^bold>v\<^bold>i\<^bold>e\<^bold>w R \<longmapsto> R\<heavy_comma> SYNTHESIS x \<Ztypecolon> Val raw T  \<^bold>@\<^bold>G\<^bold>O\<^bold>A\<^bold>L G\<close>
+  unfolding GOAL_CTXT_def
+  by (cases raw; simp add: Val_expn view_shift_id)
+
+lemma [\<phi>reason 1200 for \<open>\<^bold>v\<^bold>i\<^bold>e\<^bold>w ?S1 \<longmapsto> ?S2\<heavy_comma> SYNTHESIS ?x <val-of> (?raw::?'a sem_value) \<Ztypecolon> ?T  \<^bold>@\<^bold>G\<^bold>O\<^bold>A\<^bold>L ?G\<close>]:
+  \<open> sem_value.dest raw \<in> (x \<Ztypecolon> T)
+\<Longrightarrow> \<^bold>v\<^bold>i\<^bold>e\<^bold>w R \<longmapsto> R\<heavy_comma> SYNTHESIS x <val-of> raw \<Ztypecolon> Val raw T  \<^bold>@\<^bold>G\<^bold>O\<^bold>A\<^bold>L G\<close>
+  unfolding GOAL_CTXT_def
+  by (cases raw; simp add: Val_expn view_shift_id)
+
+lemma [\<phi>reason 1200 for \<open>\<^bold>v\<^bold>i\<^bold>e\<^bold>w ?S1 \<longmapsto> ?S2\<heavy_comma> SYNTHESIS ?x <set-to> ?raw \<Ztypecolon> ?T  \<^bold>@\<^bold>G\<^bold>O\<^bold>A\<^bold>L ?G\<close>]:
+  \<open> ERROR TEXT(\<open>Local value is immutable. Cannot assign to\<close> raw)
+\<Longrightarrow> \<^bold>v\<^bold>i\<^bold>e\<^bold>w R \<longmapsto> R\<heavy_comma> SYNTHESIS x <set-to> raw \<Ztypecolon> T  \<^bold>@\<^bold>G\<^bold>O\<^bold>A\<^bold>L G\<close>
+  by simp
+
+lemma [\<phi>reason 1500 for \<open>PROP Synthesis_by (?raw::?'a sem_value) (Trueprop (\<^bold>p\<^bold>r\<^bold>o\<^bold>c ?f \<lbrace> ?R1 \<longmapsto> \<lambda>ret. ?R2\<heavy_comma> ?x \<Ztypecolon> Val ret ?T \<^bold>t\<^bold>h\<^bold>r\<^bold>o\<^bold>w\<^bold>s ?E \<rbrace>)) \<^bold>@\<^bold>G\<^bold>O\<^bold>A\<^bold>L ?G\<close>]:
+  \<open> sem_value.dest raw \<in> (x \<Ztypecolon> T)
+\<Longrightarrow> PROP Synthesis_by raw (Trueprop (\<^bold>p\<^bold>r\<^bold>o\<^bold>c Return raw \<lbrace> R \<longmapsto> \<lambda>ret. R\<heavy_comma> x \<Ztypecolon> Val ret T \<rbrace>)) \<^bold>@\<^bold>G\<^bold>O\<^bold>A\<^bold>L G\<close>
+  for raw :: \<open>'a sem_value\<close>
+  unfolding Synthesis_by_def Action_Tag_def GOAL_CTXT_def
+            \<phi>Procedure_def Return_def det_lift_def
+  by (cases raw; simp add: Val_expn)
+
+
+
+
+
+subsubsection \<open>Auto unfolding for value list\<close>
+
+lemma [\<phi>programming_simps]:
+  \<open>(\<exists>*x. x \<Ztypecolon> Val rawv Empty_List) = (1 \<^bold>s\<^bold>u\<^bold>b\<^bold>j USELESS (rawv = \<phi>V_nil))\<close>
+  unfolding set_eq_iff USELESS_def
+  by (cases rawv; simp add: \<phi>expns)
+
+lemma [\<phi>programming_simps]:
+  \<open>(\<exists>*x. x \<Ztypecolon> Val rawv (List_Item T))
+ = (\<exists>*x. x \<Ztypecolon> Val (\<phi>V_hd rawv) T \<^bold>s\<^bold>u\<^bold>b\<^bold>j USELESS (\<exists>v. rawv = \<phi>V_cons v \<phi>V_nil))\<close>
+  unfolding set_eq_iff \<phi>V_cons_def USELESS_def
+  apply (cases rawv; clarsimp simp add: \<phi>expns \<phi>V_tl_def \<phi>V_hd_def times_list_def; rule;
+          clarsimp simp add: sem_value_All sem_value_exists)
+  by blast+
+
+lemma [simp]:
+  \<open> [] \<notin> (\<exists>*x. x \<Ztypecolon> L)
+\<Longrightarrow> ((\<exists>*x. x \<Ztypecolon> Val rawv (List_Item T \<^emph> L)) :: 'a::sep_algebra set)
+  = ((\<exists>*x. x \<Ztypecolon> Val (\<phi>V_tl rawv) L) * (\<exists>*x. x \<Ztypecolon> Val (\<phi>V_hd rawv) T))\<close>
+  unfolding set_eq_iff
+  apply (cases rawv; clarsimp simp add: \<phi>expns \<phi>V_tl_def \<phi>V_hd_def times_list_def)
+  by (metis (no_types, opaque_lifting) append_Cons append_Nil list.exhaust_sel
+            list.sel(1) list.sel(2) list.sel(3))
+
+lemma [simp]:
+  \<open>[] \<notin> (\<exists>*x. x \<Ztypecolon> (List_Item T \<^emph> L))\<close>
+  by (rule; clarsimp simp add: \<phi>expns times_list_def)
+
+lemma [simp]:
+  \<open>[] \<notin> (\<exists>*x. x \<Ztypecolon> List_Item T)\<close>
+  by (rule; clarsimp simp add: \<phi>expns times_list_def)
+
+
+
+
+end
