Phi_System/IDE_CP_Reasoning2.thy
@@ -1,0 +1,140 @@
+chapter \<open>Reasoning Processes in IDE-CP - Part I\<close>
+
+text \<open>The part includes some reasoning processes that can already be defined
+  after the IDE-CP is ready.\<close>
+
+theory IDE_CP_Reasoning2
+  imports IDE_CP
+begin
+
+section \<open>Extracts Values\<close>
+
+text \<open>The section includes several processes handling values used in different scenarios.\<close>
+
+subsection \<open>Removing Values\<close>
+
+text \<open>Given an assertion X, antecedent \<^term>\<open>Remove_Values X X'\<close>
+  returns X' where all free value assertions \<^term>\<open>x \<Ztypecolon> Val raw T\<close> filtered out, where \<^term>\<open>raw\<close>
+  contains at least one free variable of \<^typ>\<open>'a sem_value\<close>.
+
+  It is typically used in exception. When a computation triggers an exception at state X,
+    the state recorded in the exception is exactly X' where value assertions are filtered out.\<close>
+
+definition \<open>Remove_Values' (remain::assn) (keep::assn) (check::assn) (ret::assn)
+              \<longleftrightarrow> (keep = check \<longrightarrow> (remain * keep \<^bold>i\<^bold>m\<^bold>p\<^bold>l\<^bold>i\<^bold>e\<^bold>s ret))\<close>
+
+(* lemma [\<phi>reason for \<open>Remove_Values ?ex ?var_X ?Z\<close>]:
+  \<open>Remove_Values ex X X\<close>
+  unfolding Remove_Values_def using implies_refl . *)
+
+lemma [\<phi>reason 1200 for \<open>Remove_Values (ExSet ?T) ?T'\<close>]:
+  \<open>(\<And>c. Remove_Values (T c) (T' c))
+\<Longrightarrow> Remove_Values (ExSet T) (ExSet T')\<close>
+  unfolding Remove_Values_def Imply_def
+  by (simp add: \<phi>expns) blast
+
+lemma [\<phi>reason 1200 for \<open>Remove_Values (?T \<^bold>s\<^bold>u\<^bold>b\<^bold>j ?P) ?T'\<close>]:
+  \<open> Remove_Values T T'
+\<Longrightarrow> Remove_Values (T \<^bold>s\<^bold>u\<^bold>b\<^bold>j P) (T' \<^bold>s\<^bold>u\<^bold>b\<^bold>j P)\<close>
+  unfolding Remove_Values_def Imply_def
+  by (simp add: \<phi>expns)
+
+lemma [\<phi>reason 1200 for \<open>Remove_Values (?R * ?X) ?Z\<close>]:
+  \<open> Remove_Values R R'
+\<Longrightarrow> Remove_Values'  R' X X Z
+\<Longrightarrow> Remove_Values (R * X) Z\<close>
+  unfolding Remove_Values_def Imply_def Remove_Values'_def
+  by (simp add: \<phi>expns) blast
+
+lemma [\<phi>reason 1100 for \<open>Remove_Values ?R ?Z\<close>]:
+  \<open> Remove_Values'  1 R R Z
+\<Longrightarrow> Remove_Values R Z\<close>
+  unfolding Remove_Values_def Remove_Values'_def Imply_def
+  by simp
+
+lemma [\<phi>reason 1200 for \<open>Remove_Values' ?R ?Y (SYNTHESIS ?X) ?Z\<close>]:
+  \<open> Remove_Values' R Y X Z
+\<Longrightarrow> Remove_Values' R Y (SYNTHESIS X) Z\<close>
+  unfolding Remove_Values'_def Synthesis_def .
+
+(* lemma [\<phi>reason 1200 for \<open>Remove_Values' ?R ?Y (FIX ?X) ?Z\<close>]:
+  \<open> Remove_Values' R Y X Z
+\<Longrightarrow> Remove_Values' R Y (FIX X) Z\<close>
+  unfolding Remove_Values'_def Fix_def . *)
+
+lemma [\<phi>reason 1100 for \<open>Remove_Values' 1 ?Y ?X ?Z\<close>]:
+  \<open>Remove_Values' 1 Y X Y\<close>
+  unfolding Remove_Values'_def Imply_def by simp
+
+lemma Remove_Values'_accept_1[\<phi>reason 1110 for \<open>Remove_Values' 1 ?Y ?X ?Z\<close>]:
+  \<open>Remove_Values' 1 Y X Y\<close>
+  unfolding Remove_Values'_def Imply_def by simp
+
+lemma Remove_Values'_accept[\<phi>reason 1100 for \<open>Remove_Values' ?R ?Y ?X ?Z\<close>]:
+  \<open>Remove_Values' R Y X (R * Y)\<close>
+  unfolding Remove_Values'_def Imply_def by simp
+
+lemma Remove_Values'_reject_val:
+  \<open>Remove_Values' R Y (x \<Ztypecolon> Val raw T) R\<close>
+  unfolding Remove_Values'_def Imply_def by (simp add: \<phi>expns)
+
+\<phi>reasoner_ML Remove_Values'_reject_val 1200
+  (\<open>Remove_Values' ?R ?Y (?x \<Ztypecolon> Val ?raw ?T) ?Z\<close>) = \<open>
+fn (ctxt, sequent) =>
+  let
+    val Const (\<^const_name>\<open>Remove_Values'\<close>, _) $ R $ _
+          $ (Const (\<^const_name>\<open>\<phi>Type\<close>, _) $ _ $ (Const (\<^const_name>\<open>Val\<close>, _) $ raw $ _))
+          $ _ = Thm.major_prem_of sequent
+    fun has_free_val (Free (_, Type (\<^type_name>\<open>sem_value\<close>, [_]))) = true
+      | has_free_val (A $ B) = has_free_val A orelse has_free_val B
+      | has_free_val (Abs (_,_,X)) = has_free_val X
+      | has_free_val _ = false
+    val rule =
+      if has_free_val raw
+      then @{thm Remove_Values'_reject_val}
+      else (case R of Const (\<^const_name>\<open>one_class.one\<close>, _) => @{thm Remove_Values'_accept_1}
+                    | _ => @{thm Remove_Values'_accept})
+  in
+    Seq.single (ctxt, rule RS sequent)
+  end
+\<close>
+
+
+subsection \<open>Extract a Value\<close>
+
+definition \<open>Extract_a_Value (S_in::assn) S_out val_out \<longleftrightarrow> (S_in \<^bold>i\<^bold>m\<^bold>p\<^bold>l\<^bold>i\<^bold>e\<^bold>s S_out \<^bold>a\<^bold>n\<^bold>d val_out)\<close>
+
+text \<open>\<^prop>\<open>Extract_a_Value S_in S_out val_out\<close> removes the first (right-most) value from the
+  input assertion \<open>S_in\<close> and gives the specification theorem of the removed value in \<open>val_out\<close>.
+
+  The process is used during assigning a local value to a binding which
+    enables user to access the value later.
+  The specification theorem of the value is in form \<^prop>\<open>sem_value.dest raw_val \<in> (x \<Ztypecolon> T)\<close>.
+  The binding is bound with this theorem which is used when later loading this value back
+    to the state sequent when user is accessing the value.
+\<close>
+
+lemma [\<phi>reason 1200 for \<open>Extract_a_Value (?R \<heavy_comma> ?x \<Ztypecolon> \<^bold>v\<^bold>a\<^bold>l[?v] ?T) ?R ?V\<close>]:
+  \<open>Extract_a_Value (R \<heavy_comma> x \<Ztypecolon> \<^bold>v\<^bold>a\<^bold>l[v] T) R (sem_value.dest v \<in> (x \<Ztypecolon> T))\<close>
+  unfolding Extract_a_Value_def Imply_def
+  by (simp add: \<phi>expns)
+
+lemma [\<phi>reason 1100]:
+  \<open> Extract_a_Value R R' V
+\<Longrightarrow> Extract_a_Value (R\<heavy_comma> X) (R'\<heavy_comma> X) V\<close>
+  unfolding Extract_a_Value_def
+  by (rule implies_right_prod)
+
+lemma [\<phi>reason 1000]:
+  \<open> ERROR TEXT(\<open>The assertion has no value.\<close>)
+\<Longrightarrow> Extract_a_Value R R' V\<close>
+  by blast
+
+lemma apply_extract_a_value:
+  \<open> \<^bold>c\<^bold>u\<^bold>r\<^bold>r\<^bold>e\<^bold>n\<^bold>t s [R] \<^bold>r\<^bold>e\<^bold>s\<^bold>u\<^bold>l\<^bold>t\<^bold>s \<^bold>i\<^bold>n S
+\<Longrightarrow> Extract_a_Value S S' V
+\<Longrightarrow> (\<^bold>c\<^bold>u\<^bold>r\<^bold>r\<^bold>e\<^bold>n\<^bold>t s [R] \<^bold>r\<^bold>e\<^bold>s\<^bold>u\<^bold>l\<^bold>t\<^bold>s \<^bold>i\<^bold>n S') \<and> V\<close>
+  unfolding Extract_a_Value_def
+  using \<phi>cast_P .
+
+end
